update all

src/mem.v
@@ -10,12 +10,48 @@ From mathcomp Require Import ssrfun ssrbool eqtype ssrnat seq fintype finfun.
 
 Require Import bitsrep bitsops cursor pmap reader writer.
 
-Local Open Scope update_scope.
-
 Set Implicit Arguments.
 Unset Strict Implicit.
 Import Prenex Implicits.
 
+(* 256-bit addressable memory of bytes *)
+(*=Mem *)
+Definition Mem := PMAP BYTE 256.
+(*=End*)
 
+Definition PTR := EVMWORD.
+Identity Coercion PTRtoEVMWORD : PTR >-> EVMWORD.
 
+(* Initialize the memory, no memory is mapped *)
+Definition initialMemory : Mem := @EmptyPMap BYTE 256.
 
+(* Check the memory region from pointer [p] to just below pointer [p'] in [m]
+   consists exactly the bytes in [xs] *)
+Fixpoint memIs (m : Mem) (p p' : PTR) xs :=
+  if xs is x::xs then m p = Some x /\ memIs m (incB p) p' xs
+  else p = p'.
+
+(* Map memory region of 32 bytes at [p] with 1-bits *)
+Definition reserveMemory (m : Mem) (p : PTR) (c : EVMWORD) : Mem :=
+  bIterFrom p c (fun p m => m !p := ones 8) m.
+
+(* Return bytes with most-significant first *)
+Definition EVMWORDtoBytes (d : EVMWORD) : BYTE*BYTE*BYTE*BYTE*BYTE*BYTE*BYTE*BYTE*
+                                          BYTE*BYTE*BYTE*BYTE*BYTE*BYTE*BYTE*BYTE*
+                                          BYTE*BYTE*BYTE*BYTE*BYTE*BYTE*BYTE*BYTE*
+                                          BYTE*BYTE*BYTE*BYTE*BYTE*BYTE*BYTE*BYTE :=
+  split32 8 8 8 8 8 8 8 8 8 8 8 8 8 8 8 8 8 8 8 8 8 8 8 8 8 8 8 8 8 8 8 8 d.
+
+Definition isMapped (p : PTR) (ms : Mem) : bool := ms p.
+
+(* Update EVMWORD at [p] on [m] *)
+Instance MemUpdateOpsEVMWORD : UpdateOps Mem PTR EVMWORD :=
+  fun m p v =>
+    let '(b31,b30,b29,b28,b27,b26,b25,b24,b23,b22,b21,b20,b19,b18,b17,b16,
+          b15,b14,b13,b12,b11,b10,b9,b8,b7,b6,b5,b4,b3,b2,b1,b0) := EVMWORDtoBytes v in
+    m !p := b0 !incB p := b1 !incB(incB p) := b2 !incB(incB(incB p)) := b3 !incB(incB(incB(incB p))) := b4 !incB(incB(incB(incB(incB p)))) := b5 !incB(incB(incB(incB(incB(incB p))))) := b6 !incB(incB(incB(incB(incB(incB(incB p)))))) := b7 !incB(incB(incB(incB(incB(incB(incB(incB p))))))) := b8 !incB(incB(incB(incB(incB(incB(incB(incB(incB p)))))))) := b9 !incB(incB(incB(incB(incB(incB(incB(incB(incB(incB p))))))))) := b10 !incB(incB(incB(incB(incB(incB(incB(incB(incB(incB(incB p)))))))))) := b11 !incB(incB(incB(incB(incB(incB(incB(incB(incB(incB(incB(incB p))))))))))) := b12 !incB(incB(incB(incB(incB(incB(incB(incB(incB(incB(incB(incB(incB p)))))))))))) := b13 !incB(incB(incB(incB(incB(incB(incB(incB(incB(incB(incB(incB(incB(incB p))))))))))))) := b14 !incB(incB(incB(incB(incB(incB(incB(incB(incB(incB(incB(incB(incB(incB(incB p)))))))))))))) := b15 !incB(incB(incB(incB(incB(incB(incB(incB(incB(incB(incB(incB(incB(incB(incB(incB p))))))))))))))) := b16 !incB(incB(incB(incB(incB(incB(incB(incB(incB(incB(incB(incB(incB(incB(incB(incB(incB p)))))))))))))))) := b17 !incB(incB(incB(incB(incB(incB(incB(incB(incB(incB(incB(incB(incB(incB(incB(incB(incB(incB p))))))))))))))))) := b18 !incB(incB(incB(incB(incB(incB(incB(incB(incB(incB(incB(incB(incB(incB(incB(incB(incB(incB(incB p)))))))))))))))))) := b19 !incB(incB(incB(incB(incB(incB(incB(incB(incB(incB(incB(incB(incB(incB(incB(incB(incB(incB(incB(incB p))))))))))))))))))) := b20 !incB(incB(incB(incB(incB(incB(incB(incB(incB(incB(incB(incB(incB(incB(incB(incB(incB(incB(incB(incB(incB p)))))))))))))))))))) := b21 !incB(incB(incB(incB(incB(incB(incB(incB(incB(incB(incB(incB(incB(incB(incB(incB(incB(incB(incB(incB(incB(incB p))))))))))))))))))))) := b22 !incB(incB(incB(incB(incB(incB(incB(incB(incB(incB(incB(incB(incB(incB(incB(incB(incB(incB(incB(incB(incB(incB(incB p)))))))))))))))))))))) := b23 !incB(incB(incB(incB(incB(incB(incB(incB(incB(incB(incB(incB(incB(incB(incB(incB(incB(incB(incB(incB(incB(incB(incB(incB p))))))))))))))))))))))) := b24 !incB(incB(incB(incB(incB(incB(incB(incB(incB(incB(incB(incB(incB(incB(incB(incB(incB(incB(incB(incB(incB(incB(incB(incB(incB p)))))))))))))))))))))))) := b25 !incB(incB(incB(incB(incB(incB(incB(incB(incB(incB(incB(incB(incB(incB(incB(incB(incB(incB(incB(incB(incB(incB(incB(incB(incB(incB p))))))))))))))))))))))))) := b26 !incB(incB(incB(incB(incB(incB(incB(incB(incB(incB(incB(incB(incB(incB(incB(incB(incB(incB(incB(incB(incB(incB(incB(incB(incB(incB(incB p)))))))))))))))))))))))))) := b27 !incB(incB(incB(incB(incB(incB(incB(incB(incB(incB(incB(incB(incB(incB(incB(incB(incB(incB(incB(incB(incB(incB(incB(incB(incB(incB(incB(incB p))))))))))))))))))))))))))) := b28 !incB(incB(incB(incB(incB(incB(incB(incB(incB(incB(incB(incB(incB(incB(incB(incB(incB(incB(incB(incB(incB(incB(incB(incB(incB(incB(incB(incB(incB p)))))))))))))))))))))))))))) := b29 !incB(incB(incB(incB(incB(incB(incB(incB(incB(incB(incB(incB(incB(incB(incB(incB(incB(incB(incB(incB(incB(incB(incB(incB(incB(incB(incB(incB(incB(incB p))))))))))))))))))))))))))))) := b30 !incB(incB(incB(incB(incB(incB(incB(incB(incB(incB(incB(incB(incB(incB(incB(incB(incB(incB(incB(incB(incB(incB(incB(incB(incB(incB(incB(incB(incB(incB(incB p)))))))))))))))))))))))))))))) := b31.
+
+(* Update EVMWORD at [p] on [m] with fixpoint *)
+Definition updateBYTE (m : Mem) (p : PTR) (b : BYTE) : option Mem :=
+  if isMapped p m then Some (m !p := b)
+  else None.
