src/cursorprops.v
@@ -1,0 +1,24 @@
+(* Properties of Cursor *)
+
+From mathcomp Require Import all_ssreflect.
+
+Require Import nathelp.
+
+Require Import bitsrep bitsprops bitsops bitsopsprops.
+
+Require Import Coq.omega.Omega.
+
+Require Import cursor.
+
+Set Implicit Arguments.
+Unset Strict Implicit.
+Import Prenex Implicits.
+
+Lemma nextIsInc n (p q : BITS n) : next p = mkCursor q -> p+#1 = q.
+Proof.
+  rewrite /next. move => EQ.
+  case E: (p == ones n). rewrite E in EQ. done.
+  rewrite E in EQ. 
+  rewrite addB1.
+  congruence.
+Qed.
